plugins/vdm2isa/pub/recursion/README.md
@@ -1,6 +1,0 @@
-# VDM Recursive Functions in Isabelle/HOL
-
-# Paper
-
-This paper was built from Isabelle sources at `../../isa/RecursiveVDM.thy`.
-
